type_system/declarational.v
@@ -382,12 +382,12 @@ with ceq' : ctype -> ctx -> comp -> comp -> Prop :=
       (c_subs2_out c_op
         (Fun (Handle (v_shift (Handler c_r h) 1 0) c_k))
         v )
-| ηPair Γ v n c C:
-    n <= ctx_len Γ ->
-    ceq' C Γ (c_subs c n v) 
+| ηPair Γ v n c C A B:
+    n <= ctx_len Γ -> has_ctype (ctx_insert Γ (TyΠ A B) n) c C ->
+    ceq' C Γ (c_subs c n v)
       (ΠMatch v (c_subs (c_shift c 2 0) (2+n) (Pair (Var 1) (Var 0))))
-| ηSum Γ v n c C:
-    n <= ctx_len Γ ->
+| ηSum Γ v n c C A B:
+    n <= ctx_len Γ -> has_ctype (ctx_insert Γ (TyΣ A B) n) c C ->
     ceq' C Γ (c_subs c n v) 
       (ΣMatch v 
         (c_subs (c_shift c 1 0) (1+n) (Inl (Var 0))) 
